Launchbury/CorrectnessOriginal.thy
@@ -57,9 +57,9 @@ case (Application y \<Gamma> e x L \<Delta> \<Theta> z e')
     using Application.hyps(9)[OF prem1] by simp
   also have "\<dots> = (\<lbrakk> Lam [y]. e' \<rbrakk>\<^bsub>\<lbrace>\<Delta>\<rbrace>\<rho>\<^esub>) \<down>Fn (\<lbrace>\<Delta>\<rbrace>\<rho> f! x)"
     unfolding *..
-  also have "\<dots> = (Fn \<cdot> (\<Lambda> v. \<lbrakk> e' \<rbrakk>\<^bsub>(\<lbrace>\<Delta>\<rbrace>\<rho>)(y f\<mapsto> v)\<^esub>)) \<down>Fn (\<lbrace>\<Delta>\<rbrace>\<rho> f! x)"
+  also have "\<dots> = (Fn \<cdot> (\<Lambda> v. \<lbrakk> e' \<rbrakk>\<^bsub>(\<lbrace>\<Delta>\<rbrace>\<rho>)(y := v)\<^esub>)) \<down>Fn (\<lbrace>\<Delta>\<rbrace>\<rho> f! x)"
     by simp
-  also have "\<dots> = \<lbrakk> e' \<rbrakk>\<^bsub>(\<lbrace>\<Delta>\<rbrace>\<rho>)(y f\<mapsto> \<lbrace>\<Delta>\<rbrace>\<rho> f! x)\<^esub>"
+  also have "\<dots> = \<lbrakk> e' \<rbrakk>\<^bsub>(\<lbrace>\<Delta>\<rbrace>\<rho>)(y := \<lbrace>\<Delta>\<rbrace>\<rho> f! x)\<^esub>"
     by simp
   also have "\<dots> = \<lbrakk> e'[y ::= x] \<rbrakk>\<^bsub>\<lbrace>\<Delta>\<rbrace>\<rho>\<^esub>"
     by (rule arg_cong[OF ESem_subst[OF `y \<noteq> x`]])
@@ -99,13 +99,13 @@ case (Variable x e \<Gamma> L \<Delta> z)
 
   have "\<lbrace>\<Gamma>\<rbrace>\<rho> = \<lbrace>(x,e) # delete x \<Gamma>\<rbrace>\<rho>"
     by (rule HSem_reorder[OF distinctVars_map_of_delete_insert[symmetric, OF Variable(5,1)]])
-  also have "\<dots> = (\<mu> \<rho>'. (\<rho> f++\<^bsub>(heapVars (delete x \<Gamma>))\<^esub> (\<lbrace>delete x \<Gamma>\<rbrace>\<rho>'))( x f\<mapsto> \<lbrakk> e \<rbrakk>\<^bsub>\<rho>'\<^esub>))"
+  also have "\<dots> = (\<mu> \<rho>'. (\<rho> f++\<^bsub>(heapVars (delete x \<Gamma>))\<^esub> (\<lbrace>delete x \<Gamma>\<rbrace>\<rho>'))( x := \<lbrakk> e \<rbrakk>\<^bsub>\<rho>'\<^esub>))"
     by (rule iterative_HSem, simp)
-  also have "\<dots> = (\<mu> \<rho>'. (\<rho> f++\<^bsub>(heapVars (delete x \<Gamma>))\<^esub> (\<lbrace>delete x \<Gamma>\<rbrace>\<rho>'))( x f\<mapsto> \<lbrakk> e \<rbrakk>\<^bsub>\<lbrace>delete x \<Gamma>\<rbrace>\<rho>'\<^esub>))"
+  also have "\<dots> = (\<mu> \<rho>'. (\<rho> f++\<^bsub>(heapVars (delete x \<Gamma>))\<^esub> (\<lbrace>delete x \<Gamma>\<rbrace>\<rho>'))( x := \<lbrakk> e \<rbrakk>\<^bsub>\<lbrace>delete x \<Gamma>\<rbrace>\<rho>'\<^esub>))"
     by (rule iterative_HSem', simp)
   finally
   have "(\<lbrace>\<Gamma>\<rbrace>\<rho>)f|` (- ?new) = (...) f|` (- ?new)" by simp
-  also have "\<dots> = (\<mu> \<rho>'. (\<rho> f++\<^bsub>heapVars \<Delta>\<^esub> (\<lbrace>\<Delta>\<rbrace>\<rho>'))( x f\<mapsto> \<lbrakk> z \<rbrakk>\<^bsub>\<lbrace>\<Delta>\<rbrace>\<rho>'\<^esub>)) f|` (- ?new)"
+  also have "\<dots> = (\<mu> \<rho>'. (\<rho> f++\<^bsub>heapVars \<Delta>\<^esub> (\<lbrace>\<Delta>\<rbrace>\<rho>'))( x := \<lbrakk> z \<rbrakk>\<^bsub>\<lbrace>\<Delta>\<rbrace>\<rho>'\<^esub>)) f|` (- ?new)"
   proof (induction rule: parallel_fix_ind[where P ="\<lambda> x y. x f|` (- ?new) = y f|` (- ?new)"])
     case 1 show ?case by simp
   next
@@ -120,9 +120,9 @@ case (Variable x e \<Gamma> L \<Delta> z)
        and "(\<lbrace>delete x \<Gamma>\<rbrace>\<sigma>) f|` heapVars (delete x \<Gamma>) = (\<lbrace>\<Delta>\<rbrace>\<sigma>') f|` heapVars (delete x \<Gamma>)".
     thus ?case
       using subset
-      by (auto intro!: fmap_eqI simp add: lookup_fmap_add_eq lookup_fmap_upd_eq lookup_fmap_restr_eq dest: fmap_restr_eqD )
+      by (auto intro!: fmap_eqI simp add: lookup_fmap_add_eq lookup_fun_upd_eq lookup_fmap_restr_eq dest: fmap_restr_eqD )
   qed
-  also have "\<dots> = (\<mu> \<rho>'. (\<rho> f++\<^bsub>heapVars \<Delta>\<^esub> (\<lbrace>\<Delta>\<rbrace>\<rho>'))( x f\<mapsto> \<lbrakk> z \<rbrakk>\<^bsub>\<rho>'\<^esub>)) f|` (-?new)"
+  also have "\<dots> = (\<mu> \<rho>'. (\<rho> f++\<^bsub>heapVars \<Delta>\<^esub> (\<lbrace>\<Delta>\<rbrace>\<rho>'))( x := \<lbrakk> z \<rbrakk>\<^bsub>\<rho>'\<^esub>)) f|` (-?new)"
     by (rule arg_cong[OF iterative_HSem'[symmetric], OF `x \<notin> heapVars \<Delta>`])
   also have "\<dots> = (\<lbrace>(x,z) # \<Delta>\<rbrace>\<rho>)  f|` (-?new)"
     by (rule arg_cong[OF iterative_HSem[symmetric], OF `x \<notin> heapVars \<Delta>`])
