Launchbury/CorrectnessResourced.thy
@@ -52,9 +52,9 @@ case (Application y \<Gamma> e x L \<Delta> \<Theta> z e')
     by (fastforce intro: monofun_cfun_arg monofun_cfun_fun monofun_LAM)
   also have "\<dots> \<sqsubseteq> (\<Lambda> (C\<cdot>r). ((\<N>\<lbrakk> Lam [y]. e' \<rbrakk>\<^bsub>\<N>\<lbrace>\<Delta>\<rbrace>\<rho>\<^esub>) \<cdot> r \<down>CFn C_restr\<cdot>r\<cdot>(\<N>\<lbrace>\<Delta>\<rbrace>\<rho> f! x)) \<cdot> r)"
     by (intro monofun_cfun_arg monofun_cfun_fun monofun_LAM *) simp_all
-  also have "\<dots> = (\<Lambda> (C\<cdot>r). (((\<Lambda> (C \<cdot> r). CFn \<cdot> (\<Lambda> v. C_restr\<cdot>r\<cdot>(\<N>\<lbrakk> e' \<rbrakk>\<^bsub>(\<N>\<lbrace>\<Delta>\<rbrace>\<rho>)(y f\<mapsto> C_restr\<cdot>r\<cdot>v)\<^esub>)))) \<cdot> r \<down>CFn C_restr\<cdot>r\<cdot>(\<N>\<lbrace>\<Delta>\<rbrace>\<rho> f! x)) \<cdot> r)"
+  also have "\<dots> = (\<Lambda> (C\<cdot>r). (((\<Lambda> (C \<cdot> r). CFn \<cdot> (\<Lambda> v. C_restr\<cdot>r\<cdot>(\<N>\<lbrakk> e' \<rbrakk>\<^bsub>(\<N>\<lbrace>\<Delta>\<rbrace>\<rho>)(y := C_restr\<cdot>r\<cdot>v)\<^esub>)))) \<cdot> r \<down>CFn C_restr\<cdot>r\<cdot>(\<N>\<lbrace>\<Delta>\<rbrace>\<rho> f! x)) \<cdot> r)"
     by simp
-  also have "\<dots> \<sqsubseteq> (\<Lambda> (C\<cdot>r). ((CFn \<cdot> (\<Lambda> v. C_restr\<cdot>r\<cdot>(\<N>\<lbrakk> e' \<rbrakk>\<^bsub>(\<N>\<lbrace>\<Delta>\<rbrace>\<rho>)(y f\<mapsto> C_restr\<cdot>r\<cdot>v)\<^esub>))) \<down>CFn C_restr\<cdot>r\<cdot>(\<N>\<lbrace>\<Delta>\<rbrace>\<rho> f! x)) \<cdot> r)"
+  also have "\<dots> \<sqsubseteq> (\<Lambda> (C\<cdot>r). ((CFn \<cdot> (\<Lambda> v. C_restr\<cdot>r\<cdot>(\<N>\<lbrakk> e' \<rbrakk>\<^bsub>(\<N>\<lbrace>\<Delta>\<rbrace>\<rho>)(y := C_restr\<cdot>r\<cdot>v)\<^esub>))) \<down>CFn C_restr\<cdot>r\<cdot>(\<N>\<lbrace>\<Delta>\<rbrace>\<rho> f! x)) \<cdot> r)"
     apply (rule cfun_belowI)
     apply (case_tac xa, simp)
     apply simp
@@ -63,9 +63,9 @@ case (Application y \<Gamma> e x L \<Delta> \<Theta> z e')
     apply (rule monofun_cfun[OF cont2monofunE[OF _ below_C] below_C])
     apply simp
     done
-  also have "\<dots> = (\<Lambda> (C\<cdot>r). (\<N>\<lbrakk> e' \<rbrakk>\<^bsub>(\<N>\<lbrace>\<Delta>\<rbrace>\<rho>)(y f\<mapsto> C_restr\<cdot>r\<cdot>(\<N>\<lbrace>\<Delta>\<rbrace>\<rho> f! x))\<^esub>) \<cdot> r)"
+  also have "\<dots> = (\<Lambda> (C\<cdot>r). (\<N>\<lbrakk> e' \<rbrakk>\<^bsub>(\<N>\<lbrace>\<Delta>\<rbrace>\<rho>)(y := C_restr\<cdot>r\<cdot>(\<N>\<lbrace>\<Delta>\<rbrace>\<rho> f! x))\<^esub>) \<cdot> r)"
     by simp
-  also have "\<dots> \<sqsubseteq> (\<Lambda> (C\<cdot>r). (\<N>\<lbrakk> e' \<rbrakk>\<^bsub>(\<N>\<lbrace>\<Delta>\<rbrace>\<rho>)(y f\<mapsto> \<N>\<lbrace>\<Delta>\<rbrace>\<rho> f! x)\<^esub>) \<cdot> r)"
+  also have "\<dots> \<sqsubseteq> (\<Lambda> (C\<cdot>r). (\<N>\<lbrakk> e' \<rbrakk>\<^bsub>(\<N>\<lbrace>\<Delta>\<rbrace>\<rho>)(y := \<N>\<lbrace>\<Delta>\<rbrace>\<rho> f! x)\<^esub>) \<cdot> r)"
     apply (rule cont2monofunE[OF _ _]) back
     apply simp
     apply (rule cfun_belowI)
@@ -112,13 +112,13 @@ case (Variable x e \<Gamma> L \<Delta> z)
 
   have "\<N>\<lbrace>\<Gamma>\<rbrace>\<rho> = \<N>\<lbrace>(x,e) # delete x \<Gamma>\<rbrace>\<rho>"
     by (rule HSem_reorder[OF distinctVars_map_of_delete_insert[symmetric, OF Variable(5,1)]])
-  also have "\<dots> = (\<mu> \<rho>'. (\<rho> f++\<^bsub>(heapVars (delete x \<Gamma>))\<^esub> (\<N>\<lbrace>delete x \<Gamma>\<rbrace>\<rho>'))( x f\<mapsto> \<N>\<lbrakk> e \<rbrakk>\<^bsub>\<rho>'\<^esub>))"
+  also have "\<dots> = (\<mu> \<rho>'. (\<rho> f++\<^bsub>(heapVars (delete x \<Gamma>))\<^esub> (\<N>\<lbrace>delete x \<Gamma>\<rbrace>\<rho>'))( x := \<N>\<lbrakk> e \<rbrakk>\<^bsub>\<rho>'\<^esub>))"
     by (rule iterative_HSem, simp)
-  also have "\<dots> = (\<mu> \<rho>'. (\<rho> f++\<^bsub>(heapVars (delete x \<Gamma>))\<^esub> (\<N>\<lbrace>delete x \<Gamma>\<rbrace>\<rho>'))( x f\<mapsto> \<N>\<lbrakk> e \<rbrakk>\<^bsub>\<N>\<lbrace>delete x \<Gamma>\<rbrace>\<rho>'\<^esub>))"
+  also have "\<dots> = (\<mu> \<rho>'. (\<rho> f++\<^bsub>(heapVars (delete x \<Gamma>))\<^esub> (\<N>\<lbrace>delete x \<Gamma>\<rbrace>\<rho>'))( x := \<N>\<lbrakk> e \<rbrakk>\<^bsub>\<N>\<lbrace>delete x \<Gamma>\<rbrace>\<rho>'\<^esub>))"
     by (rule iterative_HSem', simp)
   finally
   have "(\<N>\<lbrace>\<Gamma>\<rbrace>\<rho>)f|` (- ?new) \<sqsubseteq> (...) f|` (- ?new)" by (rule ssubst) (rule below_refl)
-  also have "\<dots> \<sqsubseteq> (\<mu> \<rho>'. (\<rho> f++\<^bsub>heapVars \<Delta>\<^esub> (\<N>\<lbrace>\<Delta>\<rbrace>\<rho>'))( x f\<mapsto> \<N>\<lbrakk> z \<rbrakk>\<^bsub>\<N>\<lbrace>\<Delta>\<rbrace>\<rho>'\<^esub>)) f|` (- ?new)"
+  also have "\<dots> \<sqsubseteq> (\<mu> \<rho>'. (\<rho> f++\<^bsub>heapVars \<Delta>\<^esub> (\<N>\<lbrace>\<Delta>\<rbrace>\<rho>'))( x := \<N>\<lbrakk> z \<rbrakk>\<^bsub>\<N>\<lbrace>\<Delta>\<rbrace>\<rho>'\<^esub>)) f|` (- ?new)"
   proof (induction rule: parallel_fix_ind[where P ="\<lambda> x y. x f|` (- ?new) \<sqsubseteq> y f|` (- ?new)"])
     case 1 show ?case by simp
   next
@@ -133,9 +133,9 @@ case (Variable x e \<Gamma> L \<Delta> z)
        and "(\<N>\<lbrace>delete x \<Gamma>\<rbrace>\<sigma>) f|` heapVars (delete x \<Gamma>) \<sqsubseteq> (\<N>\<lbrace>\<Delta>\<rbrace>\<sigma>') f|` heapVars (delete x \<Gamma>)".
     thus ?case
       using subset
-      by (auto intro!: fmap_belowI simp add: lookup_fmap_add_eq lookup_fmap_upd_eq lookup_fmap_restr_eq elim: fmap_restr_belowD)
+      by (auto intro!: fmap_belowI simp add: lookup_fmap_add_eq lookup_fun_upd_eq lookup_fmap_restr_eq elim: fmap_restr_belowD)
   qed
-  also have "\<dots> = (\<mu> \<rho>'. (\<rho> f++\<^bsub>heapVars \<Delta>\<^esub> (\<N>\<lbrace>\<Delta>\<rbrace>\<rho>'))( x f\<mapsto> \<N>\<lbrakk> z \<rbrakk>\<^bsub>\<rho>'\<^esub>)) f|` (-?new)"
+  also have "\<dots> = (\<mu> \<rho>'. (\<rho> f++\<^bsub>heapVars \<Delta>\<^esub> (\<N>\<lbrace>\<Delta>\<rbrace>\<rho>'))( x := \<N>\<lbrakk> z \<rbrakk>\<^bsub>\<rho>'\<^esub>)) f|` (-?new)"
     by (rule arg_cong[OF iterative_HSem'[symmetric], OF `x \<notin> heapVars \<Delta>`])
   also have "\<dots> = (\<N>\<lbrace>(x,z) # \<Delta>\<rbrace>\<rho>)  f|` (-?new)"
     by (rule arg_cong[OF iterative_HSem[symmetric], OF `x \<notin> heapVars \<Delta>`])
