Launchbury/ResourcedDenotational.thy
@@ -15,7 +15,7 @@ abbreviation HSem_fempty  ("\<N>\<lbrace>_\<rbrace>"  [60] 60) where "\<N>\<lbra
 
 (* The same, but with some beta_cfun's and eta_cfuns resolved.*)
 lemma CESem_simps:
-  "\<N>\<lbrakk> Lam [x]. e \<rbrakk>\<^bsub>\<rho>\<^esub> = (\<Lambda> (C\<cdot>r). (CFn\<cdot>(\<Lambda> v. C_restr\<cdot>r\<cdot>(\<N>\<lbrakk>e\<rbrakk>\<^bsub>\<rho>(x f\<mapsto> C_restr\<cdot>r\<cdot>v)\<^esub>))))"
+  "\<N>\<lbrakk> Lam [x]. e \<rbrakk>\<^bsub>\<rho>\<^esub> = (\<Lambda> (C\<cdot>r). (CFn\<cdot>(\<Lambda> v. C_restr\<cdot>r\<cdot>(\<N>\<lbrakk>e\<rbrakk>\<^bsub>\<rho>(x := C_restr\<cdot>r\<cdot>v)\<^esub>))))"
   "\<N>\<lbrakk> App e x \<rbrakk>\<^bsub>\<rho>\<^esub>    = (\<Lambda> (C\<cdot>r). ((\<N>\<lbrakk>e\<rbrakk>\<^bsub>\<rho>\<^esub>)\<cdot>r \<down>CFn C_restr\<cdot>r\<cdot>(\<rho> f! x))\<cdot>r)"
   "\<N>\<lbrakk> Var x \<rbrakk>\<^bsub>\<rho>\<^esub>      = (\<Lambda> (C\<cdot>r). (\<rho> f! x) \<cdot> r)"
   "\<N>\<lbrakk> Let as body \<rbrakk>\<^bsub>\<rho>\<^esub> = (\<Lambda> (C \<cdot> r). (\<N>\<lbrakk>body\<rbrakk>\<^bsub>\<N>\<lbrace>asToHeap as\<rbrace>\<rho>\<^esub>) \<cdot> r)"
